hax-lib/proofs/fstar/extraction/Hax_lib.fst
@@ -2,8 +2,11 @@ module Hax_lib
 #set-options "--fuel 0 --ifuel 1 --z3rlimit 15"
 open FStar.Tactics
 
-val v_assert (p: Type0) : Pure unit (requires p) (ensures (fun x -> p))
-let v_assert (v__formula: Type0) = ()
+val v_assert (p: bool) : Pure unit (requires p) (ensures (fun x -> p))
+let v_assert (v__formula: bool) = ()
+
+val assert_prop (p: Type0) : Pure unit (requires p) (ensures (fun x -> p))
+let assert_prop (v__formula: Type0) = ()
 
 val v_assume (p: Type0) : Pure unit (requires True) (ensures (fun x -> p))
 let v_assume (v__formula: Type0) = assume v__formula
